Update OCaml and Haskell packages

haskell/zar/src/Coin.hs
@@ -1,3 +1,17 @@
+{-|
+Module      : Coin
+Description : Biased coin (Bernoulli distribution).
+Copyright   : (c) Alexander Bagnall, 2023
+License     : MIT
+Maintainer  : abagnalla@gmail.com
+Stability   : experimental
+
+This module exposes an interface for constructing biased coin samplers
+via abstractions provided by the Pipes package (Consumer, Producer,
+Pipe, Effect, see https://hackage.haskell.org/package/pipes).
+-}
+
+{-# LANGUAGE Trustworthy #-}
 module Coin (coin_consumer, coin, coin_pipe, coin_producer) where
 
 import Core
@@ -5,22 +19,54 @@ import Samplers hiding (Monad)
 
 import Pipes
 
-coin_consumer :: Monad m => Integer -> Integer -> Consumer Bool m Bool
+-- | Given Integers `num` and `denom` where 0 <= `num` <= `denom` and
+-- 0 < `denom`, create a Consumer that consumes bits (assumed to be
+-- drawn randomly from a uniform distribution) to produce a single
+-- Bool sample with Pr(True) = `num` / `denom`. The Consumer can be
+-- composed with a Producer of random bits to obtain an Effect that
+-- generates a single Bool sample.
+coin_consumer :: Monad m
+              => Integer -- ^ Numerator of bias parameter p
+              -> Integer -- ^ Denominator of bias parameter p (must be positive)
+              -> Consumer Bool m Bool -- ^ Consumer result
 coin_consumer n d =
   let MkSamplers mkCoin _ _ = samplers in
     run $ mkCoin $ qmake n d
 
-coin :: Integer -> Integer -> IO (Effect IO Bool)
+-- | Given Integers `num` and `denom` where 0 <= `num` <= `denom` and
+-- 0 < `denom`, create an Effect that generates a single Bool sample
+-- with Pr(True) = `num` / `denom`. Uses a default bit producer in the
+-- IO monad based on the PRNG provided by the mwc-random package.
+coin :: Integer -- ^ Numerator of bias parameter p 
+     -> Integer -- ^ Denominator of bias parameter p (must be positive)
+     -> IO (Effect IO Bool) -- ^ IO action that creates the Effect
 coin n d = do
   bits <- default_bit_producer
   return $ bits >-> coin_consumer n d
 
-coin_pipe :: Monad m => Integer -> Integer -> Pipe Bool Bool m ()
+-- | Given Integers `num` and `denom` where 0 <= `num` <= `denom` and
+-- 0 < `denom`, create a Pipe that consumes bits (assumed to be drawn
+-- randomly from a uniform distribution) to generate a stream of Bool
+-- samples with Pr(True) = `num` / `denom`. The Pipe can be composed
+-- with a Producer of random bits to obtain a Producer that generates
+-- a stream of Bool samples.
+coin_pipe :: Monad m
+          => Integer -- ^ Numerator of bias parameter p
+          -> Integer -- ^ Denominator of bias parameter p (must be positive)
+          -> Pipe Bool Bool m () -- ^ Pipe result
 coin_pipe n d =
   let MkSamplers mkCoin _ _ = samplers in
-    repeat_pipe $ run_pipe $ mkCoin $ qmake n d
+    run_pipe $ mkCoin $ qmake n d
 
-coin_producer :: Integer -> Integer -> IO (Producer Bool IO ())
+-- | Given Integers `num` and `denom` where 0 <= `num` <= `denom` and
+-- 0 < `denom`, create a Producer that generates a stream of Bool
+-- samples with Pr(True) = `num` / `denom`. Uses a default bit
+-- producer in the IO monad based on the PRNG provided by the
+-- mwc-random package.
+coin_producer :: Integer -- ^ Numerator of bias parameter p
+              -> Integer -- ^ Denominator of bias parameter p (must be positive)
+              -> IO (Producer Bool IO ()) -- ^ IO action that creates
+                                          -- the Producer
 coin_producer n d = do
   bits <- default_bit_producer
   return $ bits >-> coin_pipe n d
