haskell/zar/src/Core.hs
@@ -1,3 +1,25 @@
+{-|
+Module      : Core
+Description : TCB (trusted computing base).
+Copyright   : (c) Alexander Bagnall, 2023
+License     : MIT
+Maintainer  : abagnalla@gmail.com
+Stability   : experimental
+
+This module contains core definitions for the Zar verified sampling
+package including conversion functions for numeric types, pipe
+helpers, and driver code for running interaction tree samplers. This
+is essentially the TCB (trusted computing base) of the Zar
+package. The numeric conversion functions are thoroughly tested using
+QuickCheck (see the test/ directory in the the project's Github
+repository).
+
+A user of the Zar package normally does not need to use anything in
+this module directly. The high-level interface for building samplers
+is provided by the Coin, Die, and Findist modules.
+-}
+
+{-# LANGUAGE Trustworthy #-}
 module Core
     ( positive_of_integer,
       integer_of_positive,
@@ -5,7 +27,6 @@ module Core
       integer_of_z,
       run,
       run_pipe,
-      repeat_pipe,
       qmake,
       bit_producer,
       default_bit_producer
@@ -13,10 +34,14 @@ module Core
 
 import Samplers hiding (Monad)
 
+import Control.Monad.Primitive
 import Pipes
 import System.Random.MWC as MWC
 
-positive_of_integer :: Integer -> Positive
+-- | Convert Integer to Positive (the type of binary-encoded positive
+-- integers extracted from Coq).
+positive_of_integer :: Integer -- ^ Integer to convert to Positive
+                    -> Positive -- ^ Positive result
 positive_of_integer n =
   if n <= 0 then
     error $ "positive_of_integer: input must be positive, got " ++ show n
@@ -32,44 +57,74 @@ positive_of_integer n =
       else
         XI $ go $ j `div` 2
 
-integer_of_positive :: Positive -> Integer
+-- | Convert Positive to Integer.
+integer_of_positive :: Positive -- ^ Positive to convert to Integer
+                    -> Integer -- ^ Integer result
 integer_of_positive XH = 1
 integer_of_positive (XO p) = 2 * integer_of_positive p
 integer_of_positive (XI p) = 2 * integer_of_positive p + 1
 
-z_of_integer :: Integer -> Z
+-- | Convert Integer to Z (the type of binary-encoded integers
+-- extracted from Coq)
+z_of_integer :: Integer -- ^ Integer to be converted to Z
+             -> Z -- ^ Z result
 z_of_integer n | n < 0 = Zneg $ positive_of_integer $ - n
 z_of_integer n | n > 0 = Zpos $ positive_of_integer n
 z_of_integer _ = Z0
 
-integer_of_z :: Z -> Integer
+-- | Convert Z to Integer.
+integer_of_z :: Z -- ^ Z to be converted to Integer
+             -> Integer -- ^ Integer result
 integer_of_z Z0 = 0
 integer_of_z (Zpos p) = integer_of_positive p
 integer_of_z (Zneg p) = - integer_of_positive p
 
-qmake :: Integer -> Integer -> Q
+-- | Build Q (the type of rationals extracted from Coq) from numerator
+-- and denominator Integers.
+qmake :: Integer -- ^ Numerator
+      -> Integer -- ^ Denominator (must be positive)
+      -> Q -- ^ Q result
 qmake n d = Qmake (z_of_integer n) (positive_of_integer d)
 
-bit_producer :: GenIO -> Producer Bool IO a
+-- | Create a Bool Producer with from a given MWC PRNG state.
+bit_producer :: PrimMonad m
+             => Gen (PrimState m) -- ^ MWC PRNG state
+             -> Producer Bool m a -- ^ Boolean Producer using the input PRNG
 bit_producer gen = do
   b <- lift $ uniform gen
   yield b
   bit_producer gen
 
+-- | Default implementation of uniform random bit stream in the IO
+-- monad. Uses the PRNG provided by the mwc-random package.
 default_bit_producer :: IO (Producer Bool IO a)
 default_bit_producer = bit_producer <$> MWC.createSystemRandom
 
-run :: Monad m => Itree () a -> Consumer Bool m a
+-- | Construct from a given interaction tree sampler a Consumer that
+-- consumes bits (assumed to be drawn randomly from a uniform
+-- distribution) to produce a single output sample.
+run :: Monad m
+    => Itree () a -- ^ Interaction tree sampler
+    -> Consumer Bool m a -- ^ Consumer that can be composed with a
+                         -- Bool Producer to obtain an Effect with
+                         -- return type 'a'
 run t = case observe t of
   RetF x -> return x
   TauF t' -> run t'
-  VisF _ k -> await >>= run . k . unsafeCoerce
+  VisF _ k -> await >>= run . k . unsafeCoerce -- Coerce Bool to Any
 
-run_pipe :: Monad m => Itree () a -> Pipe Bool a m ()
-run_pipe t = case observe t of
-  RetF x -> yield x
-  TauF t' -> run_pipe t'
-  VisF _ k -> await >>= run_pipe . k . unsafeCoerce
-
-repeat_pipe :: Monad m => Pipe a b m r -> Pipe a b m r
-repeat_pipe pipe = pipe >> repeat_pipe pipe
+-- | Construct from a given interaction tree sampler a Pipe that
+-- consumes bits (assumed to be drawn randomly from a uniform
+-- distribution) to generate a stream of output samples.
+run_pipe :: Monad m
+         => Itree () a -- ^ Interaction tree sampler
+         -> Pipe Bool a m () -- ^ Pipe that can be composed with a
+                             -- Bool Producer to obtain a Producer
+                             -- that generates samples of type 'a'
+run_pipe t = go t >> run_pipe t
+  where
+    go :: Monad m => Itree () a -> Pipe Bool a m ()
+    go t' = case observe t' of
+             RetF x -> yield x
+             TauF t'' -> go t''
+             VisF _ k -> await >>= go . k . unsafeCoerce -- Coerce Bool to Any
