ocaml/zar/lib/die.ml
@@ -2,13 +2,13 @@ open Core
 open Samplers
 
 let cached_die : ((__, z) itree) ref =
-  ref (coin_die_samplers.die_sampler Z0)
+  ref (samplers.die_sampler Z0)
 
 let build n =
   if n <= 0 then
     raise (ZarError "Die.build: n must be positive")
   else
-    cached_die := coin_die_samplers.die_sampler (z_of_int n)
+    cached_die := samplers.die_sampler (z_of_int n)
 
 let roll () = int_of_z @@ run !cached_die
 
