ocaml/zar/lib/findist.ml
@@ -2,7 +2,7 @@ open Core
 open Samplers
 
 let cached_sampler : ((__, z) itree) ref =
-  ref (coin_die_samplers.findist_sampler [z_of_int 1])
+  ref (samplers.findist_sampler [z_of_int 1])
 
 let build weights =
   if List.exists (fun w -> w < 0) weights then
@@ -11,7 +11,7 @@ let build weights =
     raise (ZarError "Findist.weights: at least one weight must be positive")
   else
     cached_sampler :=
-      coin_die_samplers.findist_sampler @@ List.map z_of_int weights
+      samplers.findist_sampler @@ List.map z_of_int weights
 
 let sample () = int_of_z @@ run !cached_sampler
 
