tutorial.v
@@ -1,9 +1,9 @@
-(** * Tutorial. *)
+(** * Tutorial/template. *)
 
 Set Implicit Arguments.
 Set Contextual Implicit.
 
-From Coq Require Import Streams Basics QArith String Lia Lra.
+From Coq Require Import Streams Basics QArith String Lia Lqa.
 Local Open Scope program_scope.
 Local Open Scope string_scope.
 
@@ -13,38 +13,69 @@ Import ITreeNotations.
 Local Open Scope itree_scope.
 
 From zar Require Import
-  compile cotree cocwp cpGCL cpo cwp equidistribution eR misc itree order tactics tree.
+  compile cpGCL cpo cwp equidistribution eR itree misc tactics.
 Local Open Scope cpGCL_scope.
 
 (** Import pre-defined cpGCL definitions and helpers. *)
 Require Import prelude.
 
-(** Your cpGCL program. *)
-Definition prog (out : string) : cpGCL :=
-  CUniform (const 10%nat) (fun m => out <-- m).
+(** We begin with a cpGCL program to be compiled (see cpGCL.v for
+    syntax). For example, the following program implements a binomial
+    posterior with p=1/2 over variable n. Note that cpGCL values are
+    not typed (for now), so we must sometimes coerce values to the
+    intended types using functions like 'as_bool' and 'as_int' (also
+    defined in cpGCL.v). *)
+Definition prog : cpGCL :=
+  flip "b" (1#2) ;
+  "n" <-- 0%Z;
+  while (fun s => as_bool (s "b")) do
+    "n" <-- (fun s => Z.succ (as_int (s "n"))) ;
+    flip "b" (1#2)
+  end.
 
-Lemma wf_prog (out : string) :
-  wf_cpGCL (prog out).
-Proof.
-Admitted.
+(** Prove well-formedness of the program so that the equidistribution
+    theorem can be applied.*)
+Lemma wf_prog :
+  wf_cpGCL prog.
+Proof. repeat constructor; unfold const; lra. Qed.
 
+(** Here we instantiate the equidistribution theorem with the program. *)
 Section prog_equidistribution.
+  
+  (** We parameterize over a sampling environment - a record
+      containing a sequence of bitstreams and a proof that they are
+      uniformly distributed (see the definition in
+      equidistribution.v). We also parameterize over a predicate P
+      over program states and a sequence of terminal program states. *)
   Context (env : SamplingEnvironment) (P : St -> bool) (samples : nat -> St).
-  Context (out : string).
+
+  (** Suppose that each sample is the result of feeding the
+      corresponding bitstream from the sampling environment through
+      the itree compiled from the program (using the empty state). *)
   Hypothesis bitstreams_samples :
     forall i, iproduces (eq (samples i)) (env.(bitstreams) i)
-           (cpGCL_to_itree (prog out) empty).
+           (cpGCL_to_itree prog empty).
 
+  (** Then, the relative frequency of samples satisfying P (wrt. the
+      total number of samples) converges in the limit to the
+      conditional weakest pre-expectation of [fun s => if P s then 1 else
+      0] (i.e., the probability of P). *)
   Theorem prog_samples_equidistributed :
     converges (freq (is_true ∘ P) ∘ prefix samples)
-      (cwp (prog out) (fun s => if P s then 1 else 0) empty).
+      (cwp prog (fun s => if P s then 1 else 0) empty).
   Proof.
     eapply cpGCL_samples_equidistributed; eauto; apply wf_prog; auto.
   Qed.
 End prog_equidistribution.
 
-(** Extracting the sampler. *)
+(** Compile and extract itree sampler from the program to the
+    /extract/tutorial directory. We project out variable n from the
+    program state (via ITree.map) to yield a sampler with return type Z. *)
 From Coq Require Import ExtrOcamlBasic ExtrOcamlString.
 Definition sampler : itree boolE Z :=
-  ITree.map (fun s => as_int (s "out")) (cpGCL_to_itree (prog "out") empty).
+  ITree.map (fun s => as_int (s "n")) (cpGCL_to_itree prog empty).
 Extraction "extract/tutorial/prog.ml" sampler.
+
+(** Continue to /extract/tutorial/README.md for instructions on how to
+    generate and perform empirical analysis on samples from the
+    extracted itree sampler. *)
